seiostar/RQ.Metaprogram.Tests.Examples.fst
@@ -30,7 +30,7 @@ open Examples
 %splice_t[tgt13] (generate_derivation "tgt13" (`negb))
 %splice_t[tgt14] (generate_derivation "tgt14" (`if2))
 %splice_t[tgt15] (generate_derivation "tgt15" (`callback_return))
-%splice_t[tgt16] (generate_derivation "tgt16" (`callback_return'))
+// %splice_t[tgt16] (generate_derivation "tgt16" (`callback_return'))
 %splice_t[tgt16'] (generate_derivation_using "tgt16'" (`callback_return') [
   (`%identity, `tgt5)
 ])
@@ -53,13 +53,13 @@ let three_lets : bool -> unit =
 (* --- PairsSums --- *)
 
 %splice_t[tgt_make_pair] (generate_derivation "tgt_make_pair" (`make_pair))
-%splice_t[tgt_pair_of_functions] (generate_derivation "tgt_pair_of_functions" (`pair_of_functions))
+// %splice_t[tgt_pair_of_functions] (generate_derivation "tgt_pair_of_functions" (`pair_of_functions))
 %splice_t[tgt_pair_of_functions'] (generate_derivation_using "tgt_pair_of_functions'" (`pair_of_functions) [
   (`%negb, `tgt13)
 ])
-%splice_t[tgt_pair_of_functions2] (generate_derivation "tgt_pair_of_functions2" (`pair_of_functions2))
+// %splice_t[tgt_pair_of_functions2] (generate_derivation "tgt_pair_of_functions2" (`pair_of_functions2))
 
-%splice_t[tgt_pair_of_functions2'] (generate_derivation_using "tgt_pair_of_functions2'" (`pair_of_functions) [
+%splice_t[tgt_pair_of_functions2'] (generate_derivation_using "tgt_pair_of_functions2'" (`pair_of_functions2) [
   (`%negb, `tgt13);
   (`%if2, `tgt14);
 ])
@@ -81,11 +81,11 @@ let three_lets : bool -> unit =
 
 (* --- NatTopLevel --- *)
 
-%splice_t[tgt_apply_top_level_def] (generate_derivation "tgt_apply_top_level_def" (`apply_top_level_def))
+// %splice_t[tgt_apply_top_level_def] (generate_derivation "tgt_apply_top_level_def" (`apply_top_level_def))
 %splice_t[tgt_apply_top_level_def'] (generate_derivation_using "tgt_apply_top_level_def'" (`apply_top_level_def) [
   (`%thunked_id, `tgt6);
 ])
-%splice_t[tgt_apply_top_level_def2] (generate_derivation "tgt_apply_top_level_def2" (`apply_top_level_def'))
+// %splice_t[tgt_apply_top_level_def2] (generate_derivation "tgt_apply_top_level_def2" (`apply_top_level_def'))
 %splice_t[tgt_apply_top_level_def2'] (generate_derivation_using "tgt_apply_top_level_def2'" (`apply_top_level_def') [
   (`%thunked_id, `tgt6);
 ])
@@ -97,7 +97,7 @@ let three_lets : bool -> unit =
 %splice_t[tgt_nat_succ_fn] (generate_derivation "tgt_nat_succ_fn" (`nat_succ_fn))
 %splice_t[tgt_nat_add2] (generate_derivation "tgt_nat_add2" (`nat_add2))
 %splice_t[tgt_nat_five1] (generate_derivation "tgt_nat_five1" (`nat_five1))
-%splice_t[tgt_nat_five2] (generate_derivation "tgt_nat_five2" (`nat_five2))
+// %splice_t[tgt_nat_five2] (generate_derivation "tgt_nat_five2" (`nat_five2))
 %splice_t[tgt_nat_five2'] (generate_derivation_using "tgt_nat_five2'" (`nat_five2) [
   (`%nat_add2, `tgt_nat_add2)
 ])
